Launchbury/Sestoft.thy
@@ -73,4 +73,81 @@ lemma lambda_var: "map_of \<Gamma> x = Some e \<Longrightarrow> isLam e  \<Longr
   by (rule rtranclp_trans[OF r_into_rtranclp r_into_rtranclp])
      (auto intro: var\<^sub>1 var\<^sub>2)
 
+text {* An induction rule that skips the annoying case of a lambda taken off the heap *}
+
+inductive boring_step where
+  "isLam e \<Longrightarrow> boring_step (\<Gamma>, e, Upd x # S)"
+  
+
+lemma step_induction[consumes 2, case_names app\<^sub>1 app\<^sub>2 thunk lamvar var\<^sub>2 let\<^sub>1 refl trans]:
+  assumes "c \<Rightarrow>\<^sup>* c'"
+  assumes "\<not> boring_step c'"
+  assumes app\<^sub>1:  "\<And> \<Gamma> e x S . P (\<Gamma>, App e x, S)  (\<Gamma>, e , Arg x # S)"
+  assumes app\<^sub>2:  "\<And> \<Gamma> y e x S . P (\<Gamma>, Lam [y]. e, Arg x # S) (\<Gamma>, e[y ::= x] , S)"
+  assumes thunk:  "\<And> \<Gamma> x e S . map_of \<Gamma> x = Some e \<Longrightarrow> \<not> isLam e \<Longrightarrow> P (\<Gamma>, Var x, S) (delete x \<Gamma>, e , Upd x # S)"
+  assumes lamvar:  "\<And> \<Gamma> x e S . map_of \<Gamma> x = Some e \<Longrightarrow> isLam e \<Longrightarrow> P (\<Gamma>, Var x, S) ((x,e) # delete x \<Gamma>, e , S)"
+  assumes var\<^sub>2:  "\<And> \<Gamma> x e S . x \<notin> domA \<Gamma> \<Longrightarrow> isLam e \<Longrightarrow> P (\<Gamma>, e, Upd x # S) ((x,e)# \<Gamma>, e , S)"
+  assumes let\<^sub>1:  "\<And> \<Delta> \<Gamma> e S . atom ` domA \<Delta> \<sharp>* \<Gamma> \<Longrightarrow> atom ` domA \<Delta> \<sharp>* S \<Longrightarrow> P (\<Gamma>, Let \<Delta> e, S) (\<Delta>@\<Gamma>, e, S)"
+  assumes refl: "\<And> c. P c c"
+  assumes trans[trans]: "\<And> c c' c''. c \<Rightarrow>\<^sup>* c' \<Longrightarrow> c' \<Rightarrow>\<^sup>* c'' \<Longrightarrow> P c c' \<Longrightarrow> P c' c'' \<Longrightarrow> P c c''"
+  shows "P c c'"
+proof-
+  from assms(1)
+  have "P c c' \<or> (boring_step c' \<and> (\<forall> c''. c' \<Rightarrow> c'' \<longrightarrow> P c c''))"
+  proof(induction)
+  case base
+    have "P c c" by (rule refl)
+    thus ?case..
+  next
+  case (step y z)
+    from step(3)
+    show ?case
+    proof
+      assume "P c y"
+
+      note t = trans[OF `c \<Rightarrow>\<^sup>* y` r_into_rtranclp[where r = step, OF `y \<Rightarrow> z`]]
+      
+      from `y \<Rightarrow> z`
+      show ?thesis
+      proof (cases)
+        case app\<^sub>1 hence "P y z" using assms(3) by metis
+        with `P c y` show ?thesis by (metis t)
+      next
+        case app\<^sub>2 hence "P y z" using assms(4) by metis
+        with `P c y` show ?thesis by (metis t)
+      next
+        case (var\<^sub>1 \<Gamma> x e S)
+        show ?thesis
+        proof (cases "isLam e")
+          case False with var\<^sub>1 have "P y z" using assms(5) by metis
+          with `P c y` show ?thesis by (metis t)
+        next
+          case True
+          have *: "y \<Rightarrow>\<^sup>* ((x,e) # delete x \<Gamma>, e , S)" using var\<^sub>1 True lambda_var by metis
+
+          have "boring_step (delete x \<Gamma>, e, Upd x # S)" using True ..
+          moreover
+          have "P y ((x,e) # delete x \<Gamma>, e , S)" using var\<^sub>1 True assms(6) by metis
+          with `P c y` have "P c ((x,e) # delete x \<Gamma>, e , S)" by (rule trans[OF `c \<Rightarrow>\<^sup>* y` *])
+          ultimately
+          show ?thesis using var\<^sub>1(2,3) True by (auto elim!: step.cases)
+        qed
+      next
+        case var\<^sub>2 hence "P y z" using assms(7) by metis
+        with `P c y` show ?thesis by (metis t)
+      next
+        case let\<^sub>1 hence "P y z" using assms(8) by metis
+        with `P c y` show ?thesis by (metis t)
+      qed
+    next
+      assume "boring_step y \<and> (\<forall>c''. y \<Rightarrow> c'' \<longrightarrow> P c c'')"
+      with `y \<Rightarrow> z`
+      have "P c z" by blast
+      thus ?thesis..
+    qed
+  qed
+  with assms(2)
+  show ?thesis by auto
+qed
+
 end
